src/OeufProof.v
@@ -158,8 +158,6 @@ Section Simulation.
     eapply TraceSemantics.compose_forward_simulation.
     eapply Dmajortodflatmajor.fsim; try eassumption.
 
-    admit. 
-
     (* Dflatmajor to Cmajor *)
     eapply TraceSemantics.compose_forward_simulation.
     eapply Dflatmajortocmajor.fsim; try eassumption.
